Rename OOPSLA -> Presentation (back)

theories/Presentation.v
@@ -25,60 +25,733 @@ Require Import DlStalk.Sound.
 Require Import DlStalk.Compl.
 Require Import DlStalk.GenFramework.
 
-From Coq Require Import Strings.String.
 From Coq Require Import Lists.List.
 From Coq Require Import Structures.Equalities.
 Import ListNotations.
-Open Scope string_scope.
 
 Import GenServerNet.
 Import Sound.
 Import SrpcDefs.
 
+(* begin hide *)
+(* Things in here would be put in separate files; we paste them here to simplify
+the patch. Please skip to the "Introduction" section. TODO elaborate wtf this is and mention that compat.v is redunat *)
+
+Module PaperCompat.
+  Definition serv_lock (n : Name) (S : Serv) :=
+    (forall v E, ~ Deq (n, R) v (serv_i S) E) /\ (exists c, SRPC (Locked c n) (serv_p S)) /\ (serv_o S = []).
+
+  Definition dead_set (DS : list Name) N :=
+    DS <> []  /\  (forall n0, In n0 DS -> exists n1, lock N n0 n1 /\ In n1 DS).
+
+  Inductive SRPCI : SRPC_State -> Proc -> Prop :=
+  | SRPCI_R h :
+    (forall c t, h (c, t) <> None -> t = Q) ->
+    (forall c v, exists cont, h (c, Q) = Some cont /\ SRPCI (Working c) (cont v)) ->
+    SRPCI Ready (PRecv h)
+  | SRPCI_WR c v P : SRPCI (Working c) (PSend (c, R) v P)
+  | SRPCI_WT c P : SRPCI (Working c) P -> SRPCI (Working c) (STau P)
+  | SRPCI_WQ c s v P : SRPCI (Locked c s) P -> SRPCI (Working c) (PSend (s, Q) v P)
+  | SRPCI_L c s h cont :
+    (forall nc, h nc <> None -> nc = (s, R)) ->
+    (h (s, R) = Some cont) ->
+    (forall v, SRPCI (Working c) (cont v)) ->
+    SRPCI (Locked c s) (PRecv h)
+  .
+
+  CoInductive SRPCC : SRPC_State -> Proc -> Prop :=
+  | SRPCC_R P0 : (forall c v P1, P0 =(Recv (c, Q) v)=> P1 -> SRPCC (Working c) P1) -> SRPCI Ready P0 -> SRPCC Ready P0
+  | SRPCC_W c P0 :
+    (forall v P1, P0 =(Send (c, R) v)=> P1 -> SRPCC Ready P1) ->
+    (forall P1, P0 =(Tau)=> P1 -> SRPCC (Working c) P1) ->
+    (forall s v P1, P0 =(Send (s, Q) v)=> P1 -> SRPCC (Locked c s) P1) ->
+    SRPCI (Working c) P0 -> SRPCC (Working c) P0
+  | SRPCC_L c s P0 : (forall v P1, P0 =(Recv (s, R) v)=> P1 -> SRPCC (Working c) P1) -> SRPCI (Locked c s) P0 -> SRPCC (Locked c s) P0
+  .
+
+  Definition client (n : Name) (S : Serv) :=
+    (exists v, In (n, Q, v) (serv_i S)  \/ In (n, R, v) (serv_o S))
+    \/ SRPCC (Working n) (serv_p S)  \/  (exists s, SRPCC (Locked n s) (serv_p S)).
+
+
+  Definition ac (n : Name) (MN : MNet) :=
+    exists n1 n2,
+      trans_lock MN n n1
+      /\ lock MN n1 n2
+      /\ (forall n', (n' = n2 \/ trans_lock MN n' n2) -> locked (MN n') <> None)
+      /\ ( alarm (MN n) = true
+          \/ (exists n', locked (MN n) = Some n'
+                   /\ In (active_ev_of MN n' n) (mserv_q (MN n)))
+          \/ (sends_to MN n2 n1 (active_probe_of MN n))
+          \/ (exists n', lock MN n2 n'
+                   /\ In (active_ev_of MN n' n) (mserv_q (MN n2))
+                   /\ In n1 (wait (MN n2)))
+          \/ (exists n' v MQ0 MQ1,
+                lock MN n2 n'
+                /\ mserv_q (MN n2) = MQ0 ++ (active_ev_of MN n' n) :: MQ1
+                /\ In (MqRecv (n1, Q) v) MQ0)
+          \/ (exists v, In (MqRecv (n1, Q) v) (mserv_q (MN n)))
+        ).
+End PaperCompat.
+
+
+Fact serv_lock_eq : forall S n, AnySRPC_serv S -> serv_lock [n] S <-> PaperCompat.serv_lock n S.
+Proof.
+  split; intros.
+  - consider (serv_lock _ _).
+    repeat split; repeat (intros ?); simpl in *.
+    + bs (In (n, R, v) &I).
+    + eauto using lock_SRPC_Locked with LTS.
+  - destruct S.
+    consider (PaperCompat.serv_lock _ _).
+    hsimpl in *.
+    repeat split; repeat (intros ?); simpl in *; eauto with LTS.
+    assert (exists v' E, Deq (n0, R) v' serv_i0 E) by eauto using In_Deq.
+    hsimpl in *.
+    bs.
+Qed.
+
+
+Fact dead_set_eq : forall N DS, SRPC_net N -> dead_set DS N <-> PaperCompat.dead_set DS N.
+
+Proof.
+  unfold PaperCompat.dead_set.
+  split; intros; repeat constructor; intros.
+  - attac.
+  - consider (dead_set _ _).
+    consider (exists L, lock_set N L n0 /\ incl L DS).
+    unfold lock_set, lock in *.
+    consider (exists n1, serv_lock [n1] (NetMod.get n0 N)) by eauto with LTS.
+    exists n1.
+    eattac.
+  - attac.
+  - hsimpl in *.
+    consider (exists n1, lock N n n1 /\ _) by eauto.
+    exists [n1].
+    unfold incl, lock in *.
+    attac.
+Qed.
+
+
+Inductive SRPC_measure : Proc -> Prop :=
+| ms_reply n v P : SRPC_measure (PSend (n, R) v P)
+| ms_tau P : SRPC_measure P -> SRPC_measure (STau P)
+| ms_query n v P : SRPC_measure P -> SRPC_measure (PSend (n, Q) v P)
+| ms_recv h : (forall v nc cont, h nc = Some cont -> SRPC_measure (cont v)) -> SRPC_measure (PRecv h)
+.
+
+Lemma SRPCI_measure : forall srpc P, srpc <> Ready -> PaperCompat.SRPCI srpc P -> SRPC_measure P.
+Proof.
+  intros.
+  induction H0; intros; constructor; eattac.
+  specialize (H0 nc ltac:(attac)); attac.
+  rewrite H4 in H1.
+  attac.
+Qed.
+
+Lemma SRPCC_SRPCI : forall srpc P, PaperCompat.SRPCC srpc P -> PaperCompat.SRPCI srpc P.
+  intros. kill H.
+Qed.
+
+Lemma SRPCC_measure : forall srpc P, srpc <> Ready -> PaperCompat.SRPCC srpc P -> SRPC_measure P.
+  intros.
+  eauto using SRPCC_SRPCI, SRPCI_measure.
+Qed.
+
+Lemma SRPCB_measure : forall c (srpc : SRPC_Busy_State c) P, SRPC_Busy srpc P -> SRPC_measure P.
+  intros.
+  induction H; intros.
+  - destruct P0; eattac.
+    + destruct n as [n [|]].
+      * constructor; attac.
+      * constructor; attac.
+    + constructor.
+      attac.
+  - specialize (HReplyAll some_val) as [? ?]; attac.
+    constructor.
+    attac.
+Qed.
+
+
+Fact SRPCB_eq : forall P c (srpc : SRPC_Busy_State c), SRPC_Busy srpc P <-> PaperCompat.SRPCI (Busy srpc) P.
+
+Proof.
+  split; intros.
+  - induction H.
+    + destruct P0.
+      * bs.
+      * destruct n as [n [|]].
+        -- constructor.
+           eauto with LTS.
+        -- consider (c = n) by eauto with LTS.
+           constructor.
+      * bs.
+      * constructor.
+        eauto with LTS.
+    + destruct P0.
+      * specialize (HReplyAll some_val) as [? ?]; bs.
+      * specialize (HReplyAll some_val) as [? ?]; bs.
+      * specialize (HReplyAll some_val) as [? ?]; attac.
+        econstructor; eattac.
+        destruct nc.
+        destruct (handle (n, t)) eqn:?; doubt.
+        specialize (HReplyOnly (Recv (n, t) some_val) (p some_val)) as [? ?]; eattac.
+      * specialize (HReplyAll some_val) as [? ?]; bs.
+  - assert (SRPC_measure P) by (apply SRPCI_measure with (srpc:=Busy srpc); attac).
+    generalize dependent srpc.
+    induction H0; intros; consider (PaperCompat.SRPCI _ _); attac.
+    + constructor; attac.
+    + constructor; attac.
+    + constructor; attac.
+    + constructor; eattac.
+      * consider (n = (s, R)); attac.
+      * kill H1.
+        consider (n = (s, R)); attac.
+Qed.
+
+Fact SRPC_eq : forall P srpc, SRPC srpc P <-> PaperCompat.SRPCC srpc P.
+
+Proof.
+  split; intros.
+  - generalize dependent srpc P.
+    ltac1:(cofix C).
+    intros P srpc Hsrpc.
+    destruct P > [| destruct n as [n [|]] | | ]; kill Hsrpc > [|kill HBusy].
+    all: try (solve [clear C; specialize (HQueryAll some_name some_val); kill HQueryAll; bs]).
+    all: try (solve [clear C; specialize (HReplyAll some_val); kill HReplyAll; bs]).
+    + apply PaperCompat.SRPCC_W; intros; eauto.
+      econstructor.
+      eapply SRPCB_eq.
+      eapply HQuery0.
+      attac.
+    + eapply PaperCompat.SRPCC_W; intros; eauto.
+      eapply SRPCB_eq.
+      econstructor; attac.
+    + eapply PaperCompat.SRPCC_R; intros.
+      1: { specialize HQueryOnly with (a:=Recv (c, Q) v)(P1 := P1) as [? [? ?]]; eattac. }
+      econstructor; intros.
+      * destruct (handle (c, t)) eqn:?; doubt.
+        specialize HQueryOnly with (a:=Recv (c, t) some_val)(P1 := p some_val) as [? [? ?]]; eattac.
+      * specialize (HQueryAll c v) as [? ?].
+        eattac.
+        exists cont.
+        eattac.
+        specialize HQueryOnly with (a:=Recv (c, Q) v0)(P1 := cont v0) as [? [? ?]]; eattac.
+        eapply SRPCB_eq.
+        kill H1; attac.
+    + constructor; intros; eauto.
+      eapply SRPCB_eq.
+      econstructor; intros; eauto.
+    + eapply PaperCompat.SRPCC_W; intros; eauto.
+      eapply SRPCB_eq.
+      econstructor; intros; eauto.
+  - generalize dependent srpc P.
+    ltac1:(cofix C).
+    intros P srpc Hsrpc.
+    kill Hsrpc; constructor; intros; doubt.
+    + kill H0.
+      specialize (H2 c v); eattac.
+    + kill H0.
+      attac.
+      destruct n.
+      specialize H3 with (c:=n)(v:=v); attac.
+      specialize (H2 n t ltac:(attac)); attac.
+      assert (cont0 = cont). cbv in *. rewrite H3 in H4; attac.
+      subst.
+      assert (PaperCompat.SRPCC (Working n) (cont v)). apply H with (v:=v). exists (n, Q), v, cont. attac.
+      exists n, v.
+      eattac.
+    + apply SRPCB_eq.
+      eauto.
+    + eauto.
+    + eauto.
+    + eauto.
+    + eapply SRPCB_eq.
+      eauto.
+    + apply C.
+      kill H0.
+      consider ((s0, R) = (s, R)). apply H2; attac.
+      apply H in H1.
+      auto.
+Qed.
+
+
+Fact client_eq : forall n S, serv_client n S <-> PaperCompat.client n S.
+Proof.
+  unfold PaperCompat.client.
+  split; intros.
+  - consider (serv_client _ _); unfold proc_client in *; attac.
+    rewrite SRPC_eq in *.
+    destruct srpcb; eattac.
+  - destruct S.
+    destruct `(_ \/ _); hsimpl in *.
+    + destruct `(_ \/ _); eattac.
+    + destruct `(_ \/ _); eattac; rewrite <- SRPC_eq in *; eattac.
+Qed.
+
+
+Lemma KIC_lock_locked : forall n n' MN, KIC MN -> trans_lock MN n n' -> locked (MN n) <> None.
+Proof. intros. consider (trans_lock _ _ _); attac. Qed.
+Hint Resolve KIC_lock_locked : LTS.
+
+Lemma KIC_lock_locked_loop : forall n n' MN, KIC MN -> trans_lock MN n n -> trans_lock MN n n' -> locked (MN n') <> None.
+Proof. intros. assert (trans_lock MN n' n). eapply dep_loop; eauto with LTS. eapply SRPC_lock_set_uniq; eauto with LTS. eauto with LTS. Qed.
+Hint Resolve KIC_lock_locked_loop : LTS.
+
+Lemma alarm_condition_eq : forall n MN,
+    KIC MN -> trans_lock '' MN n n ->
+    alarm_condition n MN <-> PaperCompat.ac n MN.
+Proof.
+  split; intros.
+  - consider (alarm_condition _ _).
+    + consider (exists n', lock MN n n') by (consider (trans_lock MN n n); eauto with LTS).
+      exists n, n'.
+      repeat split; intros; eauto with LTS.
+      destruct `(_ = _ \/ _); subst; eauto with LTS.
+    + assert (n = m \/ (n <> m /\ trans_lock MN n m)) as [|]
+          by (smash_eq n m; destruct `(_ = _ \/ _); attac); clear H2; subst.
+      * assert (m' = self (MN m')) by attac.
+        assert (m = self (MN m)) by attac.
+        assert (locked (MN m) = Some m') by attac.
+        consider (exists m'', lock MN m' m'').
+        {
+          consider (trans_lock MN m' m). eapply dep_loop; eauto with LTS. eapply SRPC_lock_set_uniq; attac.
+          all: eauto with LTS.
+        }
+        assert (locked (MN m') = Some m'') by attac.
+        exists m, m'.
+        repeat split; intros; eauto.
+        1: { destruct `(_ = _ \/ _); subst; eauto with LTS. }
+
+        unfold sends_to, active_ev_of, active_probe_of, NetGet in *.
+        destruct (NetMod.get m' MN) as [MQ' M' S'] eqn:HMN'.
+        destruct (NetMod.get m MN) as [MQ M S] eqn:HMN.
+        assert (m = m' -> M = M' /\ MQ = MQ' /\ m' = m'') by attac.
+        clear HMN HMN'.
+        hsimpl in *; simpl in *.
+        generalize dependent M.
+        induction M'; intros.
+        -- destruct state; hsimpl in *; simpl in *.
+           consider (sends_probe _ _ _).
+           ++ right; right; right; right. eattac.
+           ++ destruct `(In _ _ \/ _).
+              ** right; right; left. exists n'. eattac.
+              ** right; right; right; left. eattac.
+        -- consider (sends_probe _ _ _); attac.
+           destruct (NAME.eq_dec (self M) (self M')); attac.
+           ++ rewrite <- e in *. clear e.
+              attac.
+              specialize IHM' with (M := M').
+              destruct IHM' as [|[|[|[|]]]]; attac.
+              right; right; left.
+              destruct `(_ \/ _); constructor; attac.
+           ++ specialize IHM' with (M := M).
+              destruct IHM' as [|[|[|[|]]]]; attac.
+              right; right; left.
+              destruct `(_ \/ _); constructor; attac.
+      * assert (m' = self (MN m')) by attac.
+        assert (m = self (MN m)) by attac.
+        assert (n = self (MN n)) by attac.
+        assert (locked (MN m) = Some m') by attac.
+        consider (exists m'', lock MN m' m'').
+        {
+          consider (trans_lock MN m' n). eapply dep_loop; eauto with LTS. eapply SRPC_lock_set_uniq; attac.
+          all: eattac.
+        }
+        assert (locked (MN m') = Some m'') by attac.
+        hsimpl in *.
+        exists m, m'.
+        repeat split; intros; eauto.
+        1: { destruct `(_ = _ \/ _); subst; eauto with LTS. }
+
+        unfold sends_to, active_ev_of, active_probe_of, NetGet in *.
+        destruct (NetMod.get n MN) as [MQ0 M0 S0] eqn:HMN0.
+        destruct (NetMod.get m' MN) as [MQ' M' S'] eqn:HMN'.
+        destruct (NetMod.get m MN) as [MQ M S] eqn:HMN.
+        assert (n = m' -> M0 = M' /\ MQ0 = MQ') by attac.
+        clear HMN HMN' HMN0.
+        hsimpl in *; simpl in *.
+        generalize dependent M0.
+        induction M'; intros.
+        -- destruct state; hsimpl in *; simpl in *.
+           consider (sends_probe _ _ _).
+           ++ right; right; right; right. eattac.
+           ++ destruct `(In _ _ \/ _).
+              ** right; right; left. exists n'. eattac.
+              ** right; right; right; left. eattac.
+        -- consider (sends_probe _ _ _); attac.
+           destruct (NAME.eq_dec (self M0) (self M')); attac.
+           ++ rewrite <- e in *. clear e.
+              attac.
+              specialize IHM' with (M0 := M').
+              destruct IHM' as [|[|[|[|]]]]; attac.
+              right; right; left.
+              destruct `(_ \/ _); constructor; attac.
+           ++ specialize IHM' with (M0 := M0).
+              destruct IHM' as [|[|[|[|]]]]; attac.
+              right; right; left.
+              destruct `(_ \/ _); constructor; attac.
+    + exists n, n'.
+      repeat split; intros; eauto with LTS.
+      destruct `(_ \/ _); subst; eauto with LTS.
+  - unfold PaperCompat.ac in *.
+    hsimpl in *.
+    consider (exists n', lock MN n n') by (consider (trans_lock MN n n); eauto with LTS).
+    destruct `(_ \/ _) as [|[|[|[|[|]]]]]; hsimpl in *; eauto with LTS.
+    + econstructor 3 with (n':=n'); eauto.
+      enough (locked (MN n) = Some n'); attac.
+    + econstructor 2 with (m:=n1)(m':=n2); eauto.
+      unfold sends_to, active_ev_of, active_probe_of, NetGet in *.
+      destruct (NetMod.get n2 MN).
+      induction mserv_m0; attac.
+      consider (sends_to_mon _ _ _); attac.
+      specialize (IHmserv_m0 ltac:(auto)).
+      econstructor 4; eattac.
+      destruct `(_ \/ _); eauto.
+    + smash_eq n n2.
+      {
+        consider (n'0 = n') by (eapply SRPC_lock_set_uniq; eattac).
+        constructor 3 with (n':=n'); eattac.
+      }
+
+      econstructor 2 with (m:=n1)(m':=n2); eauto with LTS.
+
+      assert (NoRecvR_from n'0 (mserv_q (MN n2))).
+      {
+        unfold NoRecvR_from, NetGet, lock, lock_set in *. attac.
+        destruct (NetMod.get n2 MN) as [MQ0 M0 S0] eqn:?.
+        consider (serv_lock _ (NetMod.get n2 _)). attac.
+        intros ?.
+        apply H13 with (v:=v) in H4.
+        unfold deinstr in *. rewrite NetMod.get_map in *. attac.
+        unfold serv_deinstr in *. attac.
+        destruct S0; attac.
+      }
+
+      assert (NoSends_MQ (mserv_q (MN n2))).
+      {
+        unfold NetGet, lock, lock_set in *. attac.
+        destruct (NetMod.get n2 MN) as [MQ0 M0 S0] eqn:?.
+        consider (serv_lock _ (NetMod.get n2 _)). attac.
+        apply Forall_forall. intros. destruct x; attac.
+        apply H14 with (v:=v) in H4.
+        unfold deinstr in *. rewrite NetMod.get_map in *. attac.
+        unfold serv_deinstr in *. attac.
+        destruct S0; attac.
+        apply in_split in H10; attac.
+        clear - H15.
+        induction l1; attac.
+        destruct a; attac.
+      }
+
+      assert (locked (MN n2) = Some n'0) by attac.
+      assert (self (MN n2) = n2) by attac.
+
+      unfold sends_to, active_ev_of, active_probe_of, NetGet in *.
+      hsimpl in *. simpl in *.
+      destruct (NetMod.get n2 MN) as [MQ0 M0 S0].
+      hsimpl in *; simpl in *.
+      induction M0.
+      * apply in_split in H6 as (MQ0l & MQ0r & ?); subst.
+        econstructor 2; attac.
+        intros ? ?.
+        eapply H8; eattac.
+      * hsimpl in *. simpl in *.
+        unfold Name in *; attac.
+        destruct (NameTag_eq_dec to (n1, R)),
+          (MProbe_eq_dec msg0 {| origin := n; lock_id := lock_count (Transp.Net.NetMod.get n MN) |}).
+        2,3,4: constructor 4; eattac.
+        subst.
+        constructor 3.
+    + smash_eq n n2.
+      {
+        consider (n'0 = n') by (eapply SRPC_lock_set_uniq; eattac).
+        constructor 3 with (n':=n'); eattac.
+        rewrite `(mserv_q _ = _). attac.
+      }
+
+      econstructor 2 with (m:=n1)(m':=n2); eauto with LTS.
+
+      assert (NoRecvR_from n'0 (mserv_q (MN n2))).
+      {
+        clear - H4 H6.
+        unfold active_ev_of, active_probe_of, NoRecvR_from, NetGet, lock, lock_set in *; attac.
+        destruct (NetMod.get n2 MN) as [MQ0' M0 S0] eqn:?.
+        consider (serv_lock _ (NetMod.get n2 _)).
+        attac.
+        intros ?.
+        apply H1 with (v:=v) in H4.
+        unfold deinstr in *. rewrite NetMod.get_map in *. attac.
+        unfold serv_deinstr in *. attac.
+        destruct S0; attac.
+        intros ?.
+        attac.
+        apply H1 with (v:=v) in H4.
+        unfold deinstr in *. rewrite NetMod.get_map in *. attac.
+        unfold serv_deinstr in *. attac.
+        destruct S0; attac.
+      }
+
+      assert (NoSends_MQ (mserv_q (MN n2))).
+      {
+        unfold NetGet, lock, lock_set in *. attac.
+        destruct (NetMod.get n2 MN) as [MQ0' M0 S0] eqn:?.
+        consider (serv_lock _ (NetMod.get n2 _)).
+        apply Forall_forall. intros. destruct x; attac.
+        apply H14 with (v:=v) in H4.
+        unfold deinstr in *. rewrite NetMod.get_map in *. attac.
+        unfold serv_deinstr in *. attac.
+        destruct S0; attac.
+        clear - H10 H15.
+        destruct `(_ \/ _).
+        - apply in_split in H; hsimpl in *.
+          induction l1; attac. destruct a; attac.
+        - apply in_split in H; hsimpl in *.
+          induction MQ0; attac.
+          + induction l1; eattac. destruct a; attac.
+          + destruct a; attac.
+      }
+
+      assert (locked (MN n2) = Some n'0) by attac.
+      assert (self (MN n2) = n2) by attac.
+
+      unfold sends_to, active_ev_of, active_probe_of, NetGet in *.
+      hsimpl in *. simpl in *.
+      destruct (NetMod.get n2 MN) as [MQ0' M0 S0].
+      hsimpl in *; simpl in *.
+      induction M0.
+      * apply in_split in H7 as (MQ0l & MQ0r & ?); subst.
+        econstructor 2; attac.
+        intros ? ?.
+        eapply H8; eattac.
+      * hsimpl in *. simpl in *.
+        unfold Name in *; attac.
+        destruct (NameTag_eq_dec to (n1, R)),
+          (MProbe_eq_dec msg0 {| origin := n; lock_id := lock_count (Transp.Net.NetMod.get n MN) |}).
+        2,3,4: constructor 4; eattac.
+        subst.
+        constructor 3.
+    + econstructor 2 with (m:=n1)(m':=n); eauto.
+      1: {
+        enough (serv_client n1 (NetMod.get n '' MN)). assert (well_formed MN). attac. kill H7.
+        eapply H_lock_complete. eattac.
+        unfold deinstr, serv_deinstr in *.
+        attac.
+        unfold NetGet in *.
+        destruct (NetMod.get n MN) eqn:?.
+        attac.
+      }
+
+      assert (NoRecvR_from n' (mserv_q (MN n))).
+      {
+        unfold NoRecvR_from, NetGet, lock, lock_set in *. attac.
+        destruct (NetMod.get n MN) as [MQ0 M0 S0] eqn:?.
+        consider (serv_lock _ (NetMod.get n _)). attac.
+        intros ?.
+        apply H10 with (v:=v0) in H5.
+        unfold deinstr in *. rewrite NetMod.get_map in *. attac.
+        unfold serv_deinstr in *. attac.
+        destruct S0; attac.
+      }
+
+      assert (NoSends_MQ (mserv_q (MN n))).
+      {
+        unfold NetGet, lock, lock_set in *. attac.
+        destruct (NetMod.get n MN) as [MQ0 M0 S0] eqn:?.
+        consider (serv_lock _ (NetMod.get n _)). attac.
+        apply Forall_forall. intros. destruct x; attac.
+        apply H11 with (v:=v0) in H5.
+        unfold deinstr in *. rewrite NetMod.get_map in *. attac.
+        unfold serv_deinstr in *. attac.
+        destruct S0; attac.
+        apply in_split in H7; attac.
+        clear - H12.
+        induction l1; attac.
+        destruct a; attac.
+      }
+
+      assert (locked (MN n) = Some n') by attac.
+      assert (self (MN n) = n) by attac.
+
+      unfold sends_to, active_ev_of, active_probe_of, NetGet in *.
+      hsimpl in *. simpl in *.
+      destruct (NetMod.get n MN) as [MQ0 M0 S0].
+      simpl in *.
+      induction M0.
+      * apply in_split in H4; attac.
+        econstructor 1; attac.
+        unfold NoRecvR_from in *; attac.
+        specialize (H6 v0).
+        attac.
+      * hsimpl in *. simpl in *.
+        unfold Name in *; attac.
+        destruct (NameTag_eq_dec to (n1, R)),
+          (MProbe_eq_dec msg0 {| origin := self M0; lock_id := lock_count M0 |}).
+        2,3,4: constructor 4; eattac.
+        subst.
+        constructor 3.
+Qed.
+(* end hide *)
+
 (** * Introduction *)
 
-(** This module iterates through the major theorems, lemmas, definitions and
-notations that are used in or relevant to the paper. The project uses [Ltac2] as
-the proof language. [DlStalk.Tactics] contains definitions of custom tactics. *)
+(** This file outlines the mechanised theory presented in our submission to
+OOPSLA 2025. The structure of this file closely follows how the submission is
+divided into sections. Theorems and definitions used in the submissions are
+pointed out in third-level headers. This outline works best if viewed
+interactively in a Coq/Rocq IDE, because it allows previewing context-dependent
+outputs. *)
+
+(** ** Differences *)
+(** The mechanisation introduces some concepts in a slightly different flavour,
+mostly due to quirks of the tool; we provided explanations where the connection
+might be less obvious. The most notable differences are:
+
+- We do not provide semantics for generic SRPC processes. Instead, the
+  mechanisation operates on _concrete processes_ implemented directly in Gallina
+  via coinduction. [SRPC] is then a coinductive property that asserts adherence
+  to the SRPC protocol as described in the submission.
+
+- The mechanisation does not include _casts_, and the [C] tag is non-existent.
+
+- We do not allow "no-client" (n^\bot) SRPC states. All working and locked
+  processes must handle a query from another member of the network.
+
+The lack of "clientless" SRPC states makes well-formedness much more
+restrictive. This is because each service named [n0] that is [Working n1] needs
+to be paired with an actual service [n1] that is locked on it (recall the
+equivalence between _lock_ and _client_ relations in Definition 6.4, point 2).
+Consequently, [n1] must be [Locked n2 n0] for some [n2] --- which in turn must
+be locked on [n1]. This expands endlessly, requiring the _sort_ of names to be
+infinite (otherwise we would "run out of" names for services that are neither
+ready nor locked in cycles). Our mechanisation is compatible with that
+requirement: the only restriction we put on the [Name] type is that it belongs
+to the [Set] sort and has decidable equality. This lets us model an initially
+[Working] service [n0] via an infinite stream of services transitively locked on
+[n0]. To this end, we provide an Erlang-inspired framework ([GenServerNet]) for
+modelling well-formed initial networks with [gen_server]-style services and
+initiators to engage with them as external clients. The framework is also used
+to show that our invariants are mutually sound and hold in a practical class of
+systems. See the "appendix" of this file for more details and examples. *)
 
 (** ** Axioms and other things that may appear "assumed"
 
 A couple of objects are declared as "Axioms", "Parameters", "Variables". Most of
 them are abstracting away definitions that are not relevant for the modules they
-are declared in, and are specialised later when their implementation matters ---
-for example, [MState] is irrelevant in [Transp], but is defined in [Compl]. An
-exception to this is [Val] which is never instantiated, to make sure the
-algorithm does not rely on the type of message payloads. The only thing straight
-assumed about [Val] is that it is non-empty (otherwise the model makes little
-sense), which is done via the [some_val : Val] parameter. Same holds for
-[some_name : Name].
+are declared in, and are specialised only when their implementation matters. The
+full list is attached below:
 
-In the module [DlStalk.Network] there is a module type [NET_MOD] which we use to
-model networks as "updatable functions". The interface, akin to a typical hash
-map, declares a constructor type [t], a couple of methods, and a few "axioms"
-such as [get_put_eq] saying that accessing a freshly updated service indeed
-returns that service. We left unimplemented, partially because Coq does not
-support extensionality for its built-in map data structures, which is especially
-hard to achieve without assuming the key to be an ordered type (something we did
-not want for our [Name]). However, if functional extensionality is assumed, the
-module should be easily instantiated.
+- [Val : Set] (in [DlStalk.ModelData] and [DlStalk.GenFramework]) --- The
+  message payload. Never used in the theory, instantiated to [nat] only in
+  examples for our [gen_server]-ish framework.
+
+- [valnat : Val = nat] (in [DlStalk.GenFramework]) --- Used to "forcefully"
+  instantiate [Val] to [nat] in the examples as stated above.
+
+- [some_name : Name] (in [DlStalk.Locks]) --- We assume that [Name] is
+  non-empty, otherwise the theory does not make any sense.
+
+- [some_val : Val] (in [DlStalk.Locks]) --- We assume that [Val] is non-empty.
+
+- [Msg : Set] (in [DlStalk.Model]) --- Uninstantiated probe type. Abstracted
+  where the theory does not need it.
+
+- [MState : Set] (in [DlStalk.Model]) --- Uninstantiated monitor state type.
+  Abstracted where the theory does not need it.
+
+- [mon_handle : EMsg -> MState -> MProc] (in [DlStalk.Model]) --- Uninstantiated
+  monitor algorithm function. Abstracted where the theory does not need it.
+
+- [lock_uniq : lock_uniq_type], [lock_uniq0], [lock_uniq1] (in
+  [DlStalk.NetLocks]) --- section parameter, instantiated in
+  [SRPC_lock_set_uniq].
+
+- [lock_neq_nil : lock_neq_nil_type], [lock_neq_nil0], [lock_neq_nil1] (in
+  [DlStalk.NetLocks]) --- section parameter, instantiated in
+  [SRPC_lock_set_neq_nil].
+
+- [lock_dec : lock_dec_in] (in [DlStalk.NetLocks]) --- section parameter,
+  instantiated in [well_formed_lock_dec].
+
+- [DlStalk.Network.NET_MOD] --- Abstraction of "updatable functions". The
+  interface, akin to a typical hash map, declares a constructor type [t] for the
+  collection, a couple of methods, and a few "axioms" such as [get_put_eq]
+  saying that accessing a freshly updated service indeed returns that service.
+  Note that it is a total mapping, thus for every [Name] there must be a
+  corresponding service [Serv]. We left it unimplemented because Coq standard
+  library does not offer good data structures supporting extensional equality.
 
 On top of that, we extensively use module types following the pattern proposed
 by Michael Soegtrop in
-https://coq-club.inria.narkive.com/ux8RG4m7/module-best-practices . *)
+https://coq-club.inria.narkive.com/ux8RG4m7/module-best-practices . While useful
+in code organisation, this sometimes obfuscates in-code locations of identifiers
+--- we therefore explicitly point to [.v] files where automatic navigation
+provided by [coqdoc] fails. *)
 
-(** ** Some very generic aliases *)
 
-(** Generic predicate for invariants over transitions. *)
-Print trans_invariant.
-(** Helper to mark unconditional invariants. *)
-Print always.
+(** * Correctness Criteria for Deadlock Detection Monitors in Distributed Systems *)
 
-(** * Networks of RPC Services *)
+(** We begin by introducing generic definitions and notations for labelled
+transition systems (see [DlStalk.LTS]). [LTS] is a class instantiated by almost
+all entities featuring operational semantics in the submission. We use [N0
+=(a)=> N1] to say that [N0] transitions to [N1] through some action [a].
+Similarly, [N0 =[path]=> N1] means that [N0] can reach [N1] through a sequence
+of transitions following path (a list of actions) [path]. *)
+Print LTS.
+Print ptrans.
+Locate "_ =( _ )=> _".
+Locate "_ =[ _ ]=> _".
 
-(** ** Syntax of Processes, Queues, and Services *)
 
-(** Basic (see [DlStalk.ModelData]) *)
+Module CorrectnessCriteria.
+  (** ** Transparency *)
+  (** *** _Criterion 2.1_ *)
+  (** [Net] is an _unmonitored network_, [MNet] is _monitored_. [instr] is an
+  _instrumentation_. Their definitions are discussed later in this document. We
+  use names like [ppath] to describe paths of unmonitored networks, and [mpath]
+  for monitored. *)
+
+  Definition transp_completeness (N0 : Net) (i0 : instr) :=
+    forall path N1, (N0 =[ path ]=> N1) ->
+    exists mpath (i1 : instr), (i0 N0 =[ mpath ]=> i1 N1).
+
+  Definition transp_soundness (N0 : Net) (i0 : instr) :=
+    forall mpath0 (MN1 : MNet), (i0 N0 =[ mpath0 ]=> MN1) ->
+    exists mpath1 ppath (i2 : instr) (N2 : Net),
+      (MN1 =[ mpath1 ]=> i2 N2) /\ (N0 =[ ppath ]=> N2).
+
+  (** ** Preciseness *)
+  (** *** _Criterion 2.2_ *)
+
+  Definition detect_soundness N0 (i0 : instr) :=
+    forall path' MN1 n,
+      (i0 N0 =[ path' ]=> MN1) /\ alarm (MN1 n) = true ->
+      exists DS, In n DS /\ dead_set DS (deinstr MN1).
+
+  Definition detect_completeness N0 (i0 : instr) :=
+    forall path0' (MN1 : MNet) (DS : list Name),
+      (i0 N0 =[ path0' ]=> MN1) ->
+      dead_set DS (deinstr MN1) ->
+      exists path1' (MN2 : MNet) (n : Name),
+        (MN1 =[ path1' ]=> MN2)
+        /\ In n DS /\ alarm (MN2 n) = true.
+
+  (** ** Correctness *)
+
+  Definition detect_correct (N : Net) (i : instr) :=
+      transp_completeness N i
+    /\ transp_soundness N i
+    /\ detect_completeness N i
+    /\ detect_soundness N i.
+End CorrectnessCriteria.
+
+(** * A Formal Model of Networks of RPC-Based Services *)
+
+(** ** Services: Syntax and Semantics *)
+
+(** We do not support casts, because they are irrelevant to deadlock detection
+(and the algorithm does not care about them). *)
+
 Print Tag.
 Check Q : Tag.
 Check R : Tag.
@@ -86,8 +759,8 @@ Check R : Tag.
 Check Val : Set.
 Check Name : Set.
 
-(** Process and service (see [DlStalk.Model]) *)
-Print Proc.
+(** *** _Definition 3.1_ : Services (and queues) *)
+
 Check ((_ : Que Val) : list (Name * Tag * Val)).
 
 Print Serv.
@@ -95,6 +768,137 @@ Check serv_i : Serv -> Que Val.
 Check serv_p : Serv -> Proc.
 Check serv_o : Serv -> Que Val.
 
+(** *** _Definition 3.2_ : Abstract and concrete SRPC processes, and SRPC services *)
+
+(** The mechanisation operates primarily on concrete processes ([Proc])
+programmed coinductively in Gallina (see [DlStalk.Model]). *)
+Print Proc.
+
+(** [STau], [PSend], [PRecv] are constructors of concrete processes. The first
+two are rather standard to process calculi. The receive operator is more tricky:
+to avoid explicit substitutions, it stores a semantic message selector function
+that filters received messages based on [Name] and [Tag]: if the message is
+rejected, the function returns [None]; otherwise, it returns [Some c] where [c]
+is a continuation function parameterised by the payload [Val] of the message.
+(see [DlStalk.Model]) *)
+Check STau : Proc -> Proc.
+Check PSend : (Name * Tag) -> Val -> Proc -> Proc.
+Check PRecv : ((Name * Tag) -> option (Val -> Proc)) -> Proc.
+
+(** The generic SRPC process is captured under the [SRPC_State] type (see [DlStalk.SRPC]). *)
+
+Print SRPC_State.
+Print SRPC_Busy_State.
+
+(** *** _Fig 3_ : We characterise concrete SRPC processes via a coinductive property [SRPCC]
+to describe the simulation relation, and [SRPCI] for inductive features such as
+weak termination of each query. (see [DlStalk.PresentationCompat]) *)
+
+Print PaperCompat.SRPCC.
+
+(** [[
+CoInductive SRPCC : SRPC_State -> Proc -> Prop :=
+    SRPCC_R : forall P0 : Proc,
+              (forall (c : Que.Channel.Name) (v : Que.Channel.Val)
+                 (P1 : Proc),
+               P0 =( Recv (c, Q) v )=> P1 -> SRPCC ((Working) c) P1) ->
+              SRPCI Ready P0 -> SRPCC Ready P0
+  | SRPCC_W : forall (c : Que.Channel.Name) (P0 : Proc),
+              (forall (v : Que.Channel.Val) (P1 : Proc),
+               P0 =( Send (c, R) v )=> P1 -> SRPCC Ready P1) ->
+              (forall P1 : Proc,
+               P0 =( Tau )=> P1 -> SRPCC ((Working) c) P1) ->
+              (forall (s : Que.Channel.Name) (v : Que.Channel.Val)
+                 (P1 : Proc),
+               P0 =( Send (s, Q) v )=> P1 -> SRPCC ((Locked) c s) P1) ->
+              SRPCI ((Working) c) P0 -> SRPCC ((Working) c) P0
+  | SRPCC_L : forall (c : Srpc.Locks.Proc.Que.Channel.Name)
+                (s : Que.Channel.Name) (P0 : Proc),
+              (forall (v : Que.Channel.Val) (P1 : Proc),
+               P0 =( Recv (s, R) v )=> P1 -> SRPCC ((Working) c) P1) ->
+              SRPCI ((Locked) c s) P0 -> SRPCC ((Locked) c s) P0.
+]]
+ *)
+
+Print PaperCompat.SRPCI.
+
+(** [[
+Inductive SRPCI : SRPC_State -> Proc -> Prop :=
+    SRPCI_R : forall
+                h : Srpc.Locks.Proc.Que.Channel.Name * Tag_ ->
+                    option (Que.Channel.Val -> Proc),
+              (forall (c : Srpc.Locks.Proc.Que.Channel.Name) (t : Tag_),
+               h (c, t) <> None -> t = Q) ->
+              (forall (c : Srpc.Locks.Proc.Que.Channel.Name)
+                 (v : Que.Channel.Val),
+               exists cont : Que.Channel.Val -> Proc,
+                 h (c, Q) = Some cont /\ SRPCI ((Working) c) (cont v)) ->
+              SRPCI Ready (PRecv h)
+  | SRPCI_WR : forall (c : Srpc.Locks.Proc.Que.Channel.Name)
+                 (v : Que.Channel.Val) (P : Proc),
+               SRPCI ((Working) c) (PSend (c, R) v P)
+  | SRPCI_WT : forall (c : Srpc.Locks.Proc.Que.Channel.Name) (P : Proc),
+               SRPCI ((Working) c) P ->
+               SRPCI ((Working) c) (STau P)
+  | SRPCI_WQ : forall (c s : Srpc.Locks.Proc.Que.Channel.Name)
+                 (v : Que.Channel.Val) (P : Proc),
+               SRPCI ((Locked) c s) P ->
+               SRPCI ((Working) c) (PSend (s, Q) v P)
+  | SRPCI_L : forall (c s : Srpc.Locks.Proc.Que.Channel.Name)
+                (h : Srpc.Locks.Proc.Que.Channel.Name * Tag_ ->
+                     option (Que.Channel.Val -> Proc))
+                (cont : Que.Channel.Val -> Proc),
+              (forall nc : Srpc.Locks.Proc.Que.Channel.Name * Tag_,
+               h nc <> None -> nc = (s, R)) ->
+              h (s, R) = Some cont ->
+              (forall v : Que.Channel.Val, SRPCI ((Working) c) (cont v)) ->
+              SRPCI ((Locked) c s) (PRecv h).
+]]
+ *)
+
+(** Internally, the mechanisation uses a bit more messy [SRPC] property. We
+prove both equivalent. (see [DlStalk.SRPC] and [DlStalk.PresentationCompat]). *)
+
+Print SRPC.
+Print SRPC_Busy.
+
+Check SRPC_eq : forall (P : Proc) (srpc : SRPC_State),
+    SRPC srpc P <-> PaperCompat.SRPCC srpc P.
+
+(** *** _Definition 3.4_ : Semantics of services (see [DlStalk.Que] and [DlStalk.Model]). *)
+(** Queue actions *)
+
+Print QAct.
+
+(** [[
+  Inductive QAct (E : Set) : Set :=
+    QEnq : Que.Channel.NameTag -> E -> QAct E
+  | QDeq : Que.Channel.NameTag -> E -> QAct E.
+]]
+ *)
+
+(** Generic actions used by processes, services and monitored services. [Tau] is
+opaque in the mechanisation. *)
+
+Print Act.
+
+(** [[
+Inductive Act (Payload : Set) : Set :=
+    Send : Que.Channel.NameTag -> Payload -> Act
+  | Recv : Que.Channel.NameTag -> Payload -> Act
+  | Tau : Act.
+]]
+ *)
+
+(** *** _Fig 4_ : Process Queue and Service transitions *)
+(** All are instances of the LTS class. *)
+Print ProcTrans.
+Print QTrans.
+Print STrans.
+
+Check trans_Serv : LTS PAct Serv.
+
+(** *** _Definition 3.5_ : Networks *)
 (** We abstract implementation of the network to a module type. Contrary to the
 paper, we do not use plain functions to represent networks, because that would
 require quite global extensionality which we do not need in general. (see
@@ -137,113 +941,279 @@ Check NetMod.extensionality :
   forall N0 N1,
     (forall n, NetMod.get n N0 = NetMod.get n N1) -> N0 = N1.
 
-(** ** Semantics of Processes, Queues, Services, and Networks *)
-
-(** Generic definitions (see [DlStalk.LTS]) *)
-Print LTS.
-Print ptrans.
-Locate "_ =( _ )=> _".
-Locate "_ =[ _ ]=> _".
-
-(** Actions (see [DlStalk.Que] and [DlStalk.Model]) *)
-Print Act.
-Print QAct.
-
-(** Process, Queue and Service transitions. All are instances of the LTS class.
- *)
-Print ProcTrans.
-Print QTrans.
-Print STrans.
-
-Check trans_Serv : LTS PAct Serv.
-
-(** Network transitions. [NVTrans] is used as a helper to progress nodes within
-a network (see [DlStalk.Network]) *)
+(** *** _Fig 5_ : Network semantics. *)
+(** [NVTrans] is used as a helper to progress nodes within a network (see
+[DlStalk.Network]). *)
 Print NVTrans.
 Print NTrans.
 
-(** ** Locks and Deadlocks *)
+Goal Net = NetMod.t Serv.
+Proof. reflexivity. Defined.
 
-(** Definitions used in the project *)
+(** ** Locks and Deadlocks *)
+(** *** _Definition 3.6_ : Lock (see [DlStalk.PresentationCompat]) *)
+
+Print PaperCompat.serv_lock.
+
+(** [[
+fun (n : Name) (S : Serv) =>
+    (forall (v : Val) (E : Val), ~ Deq (n, R) v (serv_i S) E)
+ /\ (exists c : Name, SRPC (Locked c n) (serv_p S))
+ /\ serv_o S = []
+]]
+ *)
+
+(** *** _Definition 3.7_ : Deadlock (see [DlStalk.PresentationCompat]) *)
+
+Print PaperCompat.dead_set.
+
+(** [[
+PaperCompat.dead_set =
+  fun (DS : Names) (N : Net) =>
+     DS <> []
+  /\ (forall n0, In n0 DS -> exists n1, lock N n0 n1 /\ In n1 DS)
+]]
+ *)
+
+(** Definitions used in the proofs are slightly different, i.e. more general to
+aim at compatibility with the OR model (see [DlStalk.Locks] and
+[DlStalk.NetLocks]). *)
 Print proc_lock.
 Print serv_lock.
 Print lock_set.
 Print lock.
 Print dead_set.
 
+(** Compatibility of project and submission definitions (for SRPC services; see
+[DlStalk.SRPCNet]). Note that [proc_lock] is more generic and uses lock lists
+--- for future compatibility with the OR model. In case of SRPC this is always a
+singleton (modulo duplicates). Additionally, [serv_lock] relies on an additional
+predicate [Decisive], which asserts that the process does not receive queries
+and responses at the same time --- in the submission, this problem is irrelevant
+as it is prevented by the syntax, thus not mentioned there to avoid confusion.
+*)
+Print Decisive.
+Check serv_lock_eq : forall S n,
+    (exists srpc, SRPC_serv srpc S) ->
+    serv_lock [n] S <-> PaperCompat.serv_lock n S.
+
+Check dead_set_eq : forall (N : Net) (DS : Names),
+    SRPC_net N ->
+    dead_set DS N <-> PaperCompat.dead_set DS N.
+
+(** *** _Lemma 3.8_ *)
 Check dead_set_invariant : forall DS, trans_invariant (dead_set DS) always.
 
+(** Compatibility of definitions between the submission and the mechanisation
+(for SRPC services; see [DlStalk.SRPCNet]). Note that [proc_lock] is more
+generic and uses lock lists --- for future compatibility with the OR model. In
+case of SRPC this is always a singleton (modulo duplicates). Additionally,
+[serv_lock] relies on an additional predicate [Decisive], which asserts that the
+process does not receive queries and responses at the same time --- in the
+submission, this problem is irrelevant as it is prevented by the syntax, thus
+not mentioned there to avoid confusion. *)
 Print Decisive.
 
-(** Deadset-cycle equivalence (see [DlStalk.NetLocks]) *)
+Check serv_lock_eq : forall S n,
+    (exists srpc, SRPC_serv srpc S) ->
+    serv_lock [n] S <-> PaperCompat.serv_lock n S.
+
+Check dead_set_eq : forall (N : Net) (DS : Names),
+    SRPC_net N ->
+    dead_set DS N <-> PaperCompat.dead_set DS N.
+
+(** * A Model of Generic Distributed Black-Box Outline Monitors *)
+
+(** ** Monitored Services and Networks *)
+
+
+(** *** _Definition 4.1_ : Monitored services (see [DlStalk.Model]) *)
+(** **** Monitor messages *)
+(** Items stored in the monitor queue. [MqProbe] is an _incoming_ probe.
+Outgoing probes are handled differently, as described below. *)
+Print EMsg.
+(** [[
+Inductive EMsg : Set :=
+    MqSend : (Name * Tag) -> Val -> EMsg
+  | MqRecv : (Name * Tag) -> Val -> EMsg
+  | MqProbe : (Name * Tag) -> MProbe' -> EMsg.
+]]
+ *)
+
+Goal MQue = list EMsg.
+Proof. reflexivity. Defined.
+
+(** **** Monitor process *)
+(** In the mechanisation, monitors do not push outgoing
+messages to the front of their queues, but instead they maintain a "monitor
+process" with two possible states: receiving ([MRecv]), when it is ready to pick
+a message from the monitor queue (equivalent to _not_ having an outgoing probe
+at the front of the queue); and sending ([MSend]), where the monitor sends a
+probe to another monitored service (equivalent to having that outgoing message
+at the front of the monitor queue). *)
+Print MProc.
+Check MRecv : MState -> MProc.
+Check MSend : (Name * Tag) -> MProbe -> MProc -> MProc.
+
+(** **** Monitored service *)
+Print MServ.
+(** Monitor queue *)
+Check mserv_q : MServ -> MQue.
+(** Monitor process / monitor state *)
+Check mserv_m : MServ -> MProc.
+(** Supervised service *)
+Check mserv_s : MServ -> Serv.
+
+(** *** _Fig 9_ : Semantics of monitored services (see [DlStalk.Model]) *)
+Print MTrans.
+
+(** *** _Definition 4.3_ : Monitored networks *)
+(** We reuse the same network model, but with monitored services.
+Internal/external actions are abstracted through a the [gen_Act] class, so
+everything connects smoothly (see [DlStalk.Network] and [DlStalk.Transp]). *)
+
+Goal MNet = NetMod.t MServ.
+Proof. reflexivity. Defined.
+
+Check (NetMod.get : Name -> MNet -> MServ).
+Check (NetMod.get : Name -> Net  -> Serv).
+
+(** ** Instrumentation of Services and Transparency *)
+
+(** *** _Definition 4.4_ : Instrumentation *)
+(** (see [DlStalk.Model] and [DlStalk.Transp]) *)
+Print mon_assg.
+Print instr.
+Check apply_instr : instr -> Net -> MNet.
+
+(** *** _Definition 4.5_ : Deinstrumentation *)
+(** [deinstr] is a _Coercion_: that means, we can apply predicates defined for
+unmonitored networks (e.g. [dead_set]) to monitored networks. In such a case,
+[deinstr] would be applied implicitly (see [DlStalk.Model] and
+[DlStalk.Transp]). *)
+Print retract_recv.
+Print retract_send.
+Print serv_deinstr.
+Print deinstr.
+
+(** *** _Proposition 4.6_ *)
+Check instr_inv : forall (i : instr) N, deinstr (i N) = N.
+
+(** *** _Definition 4.7_ : Stripping monitor actions *)
+
+Print MNAct_to_PNAct.
+(** [[
+fix MNAct_to_PNAct (ma : MNAct) :=
+  match ma with
+  | NComm n m t (MValP v) => Some (@NComm PAct _ n m t v)
+  | NTau n (MActP Tau) => Some (NTau n Tau)
+  | _ => None
+  end  : MNAct -> option PNAct.
+]]
+ *)
+
+Print MNPath_to_PNPath.
+(** [[
+fix MNPath_to_PNPath (mpath : list MNAct) : list PNAct :=
+  match mpath with
+  | [] => []
+  | ma :: mpath' =>
+      match MNAct_to_PNAct ma with
+      | None => MNPath_to_PNPath mpath'
+      | Some a => a :: MNPath_to_PNPath mpath'
+      end
+  end  : list MNAct -> list PNAct.
+]]
+ *)
+
+(** *** _Lemma 4.9_ *)
+(** We realised that proofs in the [DlStalk.Transp] module do not expose the
+fact that the path costructed in completeness is a TODO word this better and more explicit (the [MNPath_to_PNPath mpath = path] part).
+TODO mention repo and actualyl create repo  https://anonymous.4open.science/.
+
+TODO rename this to Presentation.v so _CoqProject is the same [[
+Check @transp_complete : forall path (i0 : instr) (N0 N1 : Net),
+      (N0 =[ path ]=> N1) ->
+      exists (mpath : list MNAct) (I1 : instr),
+        (i0 N0 =[ mpath ]=> I1 N1)
+        /\ MNPath_to_PNPath mpath = path.
+]] *)
+
+(** *** _Theorem 4.8_ : Transparency --- completeness *)
+Lemma oopsla_transp_completeness : forall N0 i0,
+    CorrectnessCriteria.transp_completeness N0 i0.
+
+Proof.
+  unfold CorrectnessCriteria.transp_completeness.
+  intros.
+  specialize @transp_complete with (I0:=i0)(path:=path)(N0:=N0)(N1:=N1)
+    as (mpath & i1 & ?); attac.
+Qed.
+
+(** *** _Lemma 4.12_ *)
+(** We first prove that a path of *any* monitored network is replicable after
+deinstrumentation. *)
+Check MNPath_do : forall (mpath : list (NAct (Act:=MAct))) (MN0 MN1 : MNet),
+    MN0 =[ mpath ]=> MN1 -> deinstr MN0 =[ mpath ]=> deinstr MN1.
+
+(** We now show the statement from the submission. *)
+
+Goal forall (N0 : Net) (i0 : instr) mpath0 (MN1 : MNet),
+    (i0 N0 =[ mpath0 ]=> MN1) ->
+    exists mpath1 (i2 : instr) (N2 : Net),
+      (MN1 =[ mpath1 ]=> i2 N2)
+    /\ (N0 =[ MNPath_to_PNPath (mpath0 ++ mpath1) ]=> N2).
+Proof.
+  intros.
+  specialize @transp_sound_instr with (mnpath0:=mpath0)(I0:=i0)(N0:=N0)(MN1:=MN1)
+    as (mpath1 & ppath & i2 & N2 & ? & ?); auto.
+  exists mpath1, i2, N2.
+  split; auto.
+  assert (deinstr (i0 N0) =[mpath0 ++ mpath1]=> deinstr (i2 N2))
+    by eauto using MNPath_do with LTS.
+  repeat (rewrite instr_inv in * ).
+  remember (mpath0 ++ mpath1) as mpath; clear Heqmpath.
+  clear - H2.
+  generalize dependent N0.
+  induction mpath; attac.
+  apply IHmpath in H3.
+  consider (N0 =(a)=> N1); attac.
+  - destruct_ma a0; eattac.
+    apply path_seq1 with (middle:=(NetMod.put n &S N0)); attac.
+  - destruct v; attac.
+    apply path_seq1 with (middle:=(NetMod.put n' &S (NetMod.put n &S0 N0))); eattac.
+    econstructor; eattac.
+Qed.
+
+
+(** *** _Theorem 4.11_ : Transparency --- soundness *)
+Lemma oopsla_transp_soundness : forall N0 i0,
+    CorrectnessCriteria.transp_soundness N0 i0.
+
+Proof.
+  unfold CorrectnessCriteria.transp_soundness.
+  intros.
+  eauto using transp_sound_instr.
+Qed.
+
+(** * A Distributed Black-Box Monitoring Algorithm for Deadlock Detection *)
+
+(** *** _Proposition 5.1_ : Deadset-cycle equivalence (see [DlStalk.NetLocks]) *)
 Check dead_set_cycle : forall N : Net,
     lock_uniq_type N -> lock_neq_nil_type N -> locks_dec_in N ->
     forall DS, dead_set DS N -> exists n, In n DS /\ trans_lock N n n.
+
 Check cycle_dead_set : forall N : Net,
     lock_uniq_type N -> lock_neq_nil_type N ->
     forall n, trans_lock N n n -> exists DS, In n DS /\ dead_set DS N.
 
-(** Well formed SRPC networks fulfill the prerequisites for dead_set-cycle
-equivalence. (see [DlStalk.SRPCNet]) *)
-Import SrpcNet.
-Check SRPC_lock_set_uniq : forall [N : Net],
-    SRPC_net N ->
-    lock_uniq_type N.
-Check SRPC_lock_set_neq_nil : forall [N : Net],
-    SRPC_net N ->
-    lock_neq_nil_type N.
-Print locks_dec_in.
-Check well_formed_lock_dec :
-  forall (N : Net) n0 n1,
-    well_formed N ->
-    lock N n0 n1 \/ ~ lock N n0 n1.
 
-(** ** Single-Threaded RPC (SRPC) Services *)
-
-(** We define SRPC as a co-inductive property of processes (see [DlStalk.SRPC]) *)
-Print SRPC_State.
-Print SRPC_Busy_State.
-
-(** ** A Coq Framework for Modelling Erlang/OTP-Style SRPC Networks *)
-
-Section Framework.
-  Import GenServerNet.
-  Import Sound.
-  Import SrpcDefs.
-
-  (** Types for generic network configuration (see [DlStalk.GenFramework]) *)
-  Print ServiceConf.
-  Print InitConf.
-  Print NetConf.
-
-  (** The network is SRPC! *)
-  Check gen_net_SRPC : forall conf n,
-    exists srpc, SRPC_serv srpc (NetMod.get n (gen_net conf)).
-
-  (** Example services and network *)
-  Print echo.
-  Print fwd_service.
-  Print example_net.
-
-  (** Can deadlock *)
-  Check can_deadlock : exists path N,
-      (example_net =[ path ]=> N) /\ dead_set ["A"; "B"; "C"; "D"]%list N.
-End Framework.
-
-(** * Monitors, Instrumentation, and Transparency *)
-
-(** Probes. [MProbe] is an alias for a slightly more generic [MProbe'] (see
-[DlStalk.Compl]) *)
-Locate MProbe.
-Print MProbe'.
-Check origin  : MProbe -> Name.
-Check lock_id : MProbe -> nat.
-
-(** Monitor messages (stored in the monitor queue) (see [DlStalk.Model]) *)
-Print EMsg.
-Locate MQue.
-
-(** Monitor state (see [DlStalk.Compl]) *)
+(** *** _Definition 5.2_ Implementation of the algorithm (see [DlStalk.Compl])
+*)
+(** **** Monitor state (see [DlStalk.Compl]). *)
+(** We implement "fresh probes" by storing the name of the originator ([self]
+becomes [origin]) and counting how many times the service has been locked
+([lock_count] becomes [lock_id]). *)
 Locate MState.
 Print MState'.
 Check self       : MState -> Name.
@@ -252,74 +1222,38 @@ Check wait       : MState -> list Name.
 Check lock_count : MState -> nat.
 Check alarm      : MState -> bool.
 
-(** Monitor process (see [DlStalk.Model]) *)
-Print MProc.
-Check MRecv : MState -> MProc.
-Check MSend : (Name * Tag) -> MProbe -> MProc -> MProc.
+(** **** Probes *)
+(** [MProbe] is an alias for a slightly more generic [MProbe'] (see
+[DlStalk.Compl]) *)
+Locate MProbe.
+Print MProbe'.
+Check origin  : MProbe -> Name.
+Check lock_id : MProbe -> nat.
 
-(** Monitored service (see [DlStalk.Model]) *)
-Print MServ.
-Check mserv_q : MServ -> MQue.
-Check mserv_m : MServ -> MProc.
-Check mserv_s : MServ -> Serv.
-
-(** Transition of monitored services (see [DlStalk.Model]) *)
-Print MTrans.
-
-(** Instrumentation (see [DlStalk.Model]) *)
-Print mon_assg.
-Print instr.
-Check apply_instr : instr -> Net -> MNet.
-
-(** De-instrumentation (see [DlStalk.Model]) *)
-Print retract_recv.
-Print retract_send.
-Print serv_deinstr.
-Print deinstr.
-
-Check instr_inv : forall (i : instr) N, deinstr (i N) = N.
-
-(** Networks are generic, thus work for monitored services too (see [DlStalk.Network] and [DlStalk.Transp]) *)
-Check (NetMod.get : Name -> MNet -> MServ).
-Check (NetMod.get : Name -> Net  -> Serv).
-
-(** Transparency (see [DlStalk.Transp]) *)
-Check transp_sound : forall mnpath (MN0 MN1 : MNet),
-    MN0 =[ mnpath ]=> MN1 -> exists pnpath, deinstr MN0 =[ pnpath ]=> deinstr MN1.
-Check @transp_complete : forall path (i0 : instr) (N0 N1 : Net),
-    N0 =[ path ]=> N1 -> exists mpath (i1 : instr), i0 N0 =[ mpath ]=> i1 N1.
-
-
-(** * Black-Box Distributed Deadlock Detection Algorithm *)
-
-Module Type Alg. (* We need to backdoor it a bit... *)
+Module Type Alg.
+  (* It needs to be a bit backdoored to instantiate abstract parameters *)
   Declare Module Conf : DETECT_CONF.
   Declare Module Params : MON_PARAMS(Conf).
   Include Mh(Conf)(Params).
 
-  (** Implementation of the algorithm (see [DlStalk.Compl]) *)
+  (** **** The algorithm *)
   Check mon_handle : EMsg -> MState -> MProc.
   Print mon_handle.
 End Alg.
 
-(** * Correctness of Black-Box Distributed Deadlock Detection *)
+(** * Proving the Preciseness of Our Distributed Deadlock Detection Monitors *)
 
-(** ** Monitor Correctness Criteria *)
+(** ** Invariant Properties of Well-Formed SRPC Networks *)
 
-Section Correct.
-  Import GenServerNet.
+(** *** _Definition 6.2_ : The client relation *)
+(** (see [DlStalk.NetLocks] and [DlStalk.PresentationCompat] for compatibility
+lemmas) *)
+Print PaperCompat.client.
+Print serv_client.
+Check client_eq : forall n S, serv_client n S <-> PaperCompat.client n S.
 
-  (** Definition of correctness (see [DlStalk.GenFramework]) *)
-  Print detect_sound.
-  Print detect_complete.
-  Print detect_correct.
-End Correct.
-
-(** ** Invariants *)
-
-(** *** Well-Formed SRPC Networks  *)
-
-(**  Well-formedness at the greatest detail (see [DlStalk.SRPCNet]) *)
+(** *** _Definition 6.3_ : Well-formedness *)
+(** (see [DlStalk.SRPCNet]) *)
 Print service_wf.
 
 Check service_wf_SRPC_inv : forall [srpc : SRPC_State] [S],
@@ -382,11 +1316,77 @@ Check service_wf_c_excl_R_inv : forall [srpc : SRPC_State] [c v I P O],
     proc_client c P ->
     ~ In (c, R, v) O.
 
+(** *** _Definition 6.4_ *)
 Print well_formed.
+
+(** *** _Theorem 6.5_ *)
 Check well_formed_invariant : trans_invariant well_formed always.
 
-(** *** Sound lock knowledge  *)
+(** ** Monitor Knowledge Invariant for Complete Deadlock Detection  *)
+(** (see [DlStalk.Compl]) *)
 
+Print sends_probe.
+
+(** *** _Definition 6.8_ *)
+
+Print PaperCompat.ac.
+
+(** [[
+PaperCompat.ac =
+fun (n : Name) (MN : MNet) =>
+exists (n1 : Name) (n2 : Que.Channel.Name),
+  trans_lock '' MN n n1 /\
+  lock '' MN n1 n2 /\
+  (forall n' : Que.Channel.Name,
+   n' = n2 \/ trans_lock '' MN n' n2 -> locked (MN n') <> None) /\
+  (alarm (MN n) = true \/
+   (exists n' : DetConf.NAME.t',
+      locked (MN n) = Some n' /\ In (active_ev_of MN n' n) (mserv_q (MN n))) \/
+   sends_to MN n2 n1 (active_probe_of MN n) \/
+   (exists n' : Que.Channel.Name,
+      lock '' MN n2 n' /\
+      In (active_ev_of MN n' n) (mserv_q (MN n2)) /\ In n1 (wait (MN n2))) \/
+   (exists
+      (n' : Que.Channel.Name) (v : Mon.Proc.Que.Channel.Val)
+    (MQ0 MQ1 : MQue),
+      lock '' MN n2 n' /\
+      mserv_q (MN n2) = MQ0 ++ active_ev_of MN n' n :: MQ1 /\
+      In (MqRecv (n1, Q) v) MQ0) \/
+   (exists v : Mon.Proc.Que.Channel.Val,
+      In (MqRecv (n1, Q) v) (mserv_q (MN n))))
+     : Name -> MNet -> Prop
+]]
+ *)
+
+(** The definition used in the mechanisation is slightly different, but we show
+them equivalent for deadlocked processes in [KIC] networks (the only place where
+it is used). *)
+
+Print alarm_condition.
+
+Check alarm_condition_eq : forall (n : Name) (MN : MNet),
+    KIC MN -> trans_lock '' MN n n ->
+    alarm_condition n MN <-> PaperCompat.ac n MN.
+
+(** *** _Definition 6.7_ *)
+Print KIC.
+
+(** *** _Lemma 6.9_ *)
+Check ac_to_alarm : forall MN0 n,
+    KIC MN0 ->
+    alarm_condition n MN0 ->
+    trans_lock '' MN0 n n ->
+    exists DS mpath MN1,
+      (MN0 =[ mpath ]=> MN1)
+      /\ dead_set DS '' MN0
+      /\ detect_path DS mpath
+      /\ alarm (MN1 n) = true.
+
+(** *** _Theorem 6.10_ *)
+Check KIC_invariant : trans_invariant KIC always.
+
+
+(** ** Monitor Knowledge Invariant for Sound Deadlock Detection  *)
 (** (see [DlStalk.Sound]) *)
 Print sends_to.
 Print sends_to_mon.
@@ -396,6 +1396,7 @@ Check stm_seek : forall n nc' p p' M,
     sends_to_mon M n p ->
     sends_to_mon (MSend nc' p' M) n p.
 
+(** *** _Definition 6.11_ *)
 Print KIS.
 
 Check KIS_well_formed : forall [MN], KIS MN -> well_formed '' MN.
@@ -435,33 +1436,21 @@ Check KIS_alarm : forall [MN],
       alarm (MN n) = true ->
       trans_lock '' MN n n.
 
+(** Monitor message (in monitor queue) holding an active probe *)
+Print active_ev_of.
+
+(** *** _Theorem 6.12_ *)
 Check KIS_invariant : trans_invariant KIS always.
+
+(** ** Deadlock Detection Preciseness Result *)
+
+(** *** _Theorem 6.13_ *)
+
 Check KIS_detection_sound : forall (i0 : instr) N0 MN1 mpath n,
     KIS (i0 N0) -> (i0 N0 =[ mpath ]=> MN1) ->
     alarm (MN1 n) = true ->
     exists DS, dead_set DS '' MN1 /\ In n DS.
 
-(** Monitor message (in monitor queue) holding an active probe *)
-Print active_ev_of.
-
-(** *** Complete lock knowledge  *)
-
-(**  (see [DlStalk.Compl]) *)
-
-Print sends_probe.
-Print alarm_condition.
-Print KIC.
-
-Check KIC_invariant : trans_invariant KIC always.
-Check ac_to_alarm : forall MN0 n,
-    KIC MN0 ->
-    alarm_condition n MN0 ->
-    trans_lock '' MN0 n n ->
-    exists DS mpath MN1,
-      (MN0 =[ mpath ]=> MN1)
-      /\ dead_set DS '' MN0
-      /\ detect_path DS mpath
-      /\ alarm (MN1 n) = true.
 
 Check KIC_detection_complete : forall (i0 : instr) N0 MN1 mpath0 DS,
     KIC (i0 N0) ->
@@ -470,31 +1459,199 @@ Check KIC_detection_complete : forall (i0 : instr) N0 MN1 mpath0 DS,
     exists mpath1 MN2 n,
       (MN1 =[ mpath1 ]=> MN2) /\ In n DS /\ alarm (MN2 n) = true.
 
-(** ** Correctness *)
 
-Section Correct.
-  Import GenServerNet. Import Sound.
+Lemma oopsla_detect_soundness : forall (i0 : instr) N0,
+  KIS (i0 N0) -> CorrectnessCriteria.detect_soundness N0 i0.
 
-  (** The framework is correct (see [DlStalk.GenFramework]) *)
-  Print gen_instr.
+Proof.
+  unfold CorrectnessCriteria.detect_soundness; intros.
+  specialize KIS_detection_sound
+    with (i0:=i0)(N0:=N0)(MN1:=MN1)(n:=n)(mpath:=path')
+    as (mpath1 & MN2 & n'); attac.
+Qed.
 
+Lemma oopsla_detect_completeness : forall (i0 : instr) N0,
+    KIC (i0 N0) -> CorrectnessCriteria.detect_completeness N0 i0.
+
+Proof.
+  unfold CorrectnessCriteria.detect_completeness; intros.
+  specialize KIC_detection_complete
+    with (i0:=i0)(N0:=N0)(MN1:=MN1)(mpath0:=path0')(DS:=DS)
+    as (mpath1 & MN2 & n'); eauto.
+Qed.
+
+(** Finally, total correctness. *)
+
+Lemma oopsla_correct : forall (i0 : instr) N0,
+    KIC (i0 N0) -> KIS (i0 N0) -> CorrectnessCriteria.detect_correct N0 i0.
+
+Proof.
+  unfold CorrectnessCriteria.detect_correct; intros.
+  repeat split;
+    eauto using
+      oopsla_transp_soundness,
+      oopsla_transp_completeness,
+      oopsla_detect_soundness,
+      oopsla_detect_completeness.
+Qed.
+
+(** Assumptions are described in the introduction. In the final result, only
+[Val], [some_val], [some_name] and [NetMod] are left declared. *)
+Print Assumptions oopsla_correct.
+
+
+(** * Appendix: A Coq Framework for Modelling Erlang/OTP-Style SRPC Networks *)
+
+(** _Contents of this section are not addressed in the submission_ *)
+
+(** Proving implementation of actual Erlang code is a daunting task. Instead, we
+prove that the premises of our theory are sound and applicable by we providing a
+Coq framework for modelling networks of SRPC services in the style of
+[gen_server]s. Networks are assembled by assigning names (as strings) to
+services. All services begin as [Ready] with empty input and output queues. The
+network can start progressing via one or more _initiators_, which act as
+external clients that send queries to the services. *)
+
+Section Framework. 
+  Import String.
+  Open Scope string.
+
+  (** Services are implemented through the [ServiceConf] record: the [state_t]
+      field describes the type of internal state of the service (which can
+      differ among services); [init] is the initial state; [handle_call]
+      (following the convention from Erlang) describes how the service reacts to
+      a query [msg] received [from] a certain sender while in a given [state].
+
+      Initiators are anonymous and set [from] to [None]. For a regular service
+      named [n] it is set to [Some n])
+
+      The return type of [handle_call] is an opaque [Handler] which represents
+      SRPC-compliant code of the handling function; to construct it, we provide
+      the programmer with auxiliary syntax (discussed below). *)
+
+  Print ServiceConf.
+
+  (** [[
+      Record ServiceConf : Type := sconf
+      { state_t : Set;
+        init : state_t;
+        handle_call : option string -> Val -> state_t -> Handler state_t
+      }.
+      ]]
+   *)
+
+  (** The simplest SRPC service is [echo] defined below, which handles queries
+      by immediately replying with the message it received. In [handle_call],
+      the auxiliary syntax [reply msg state] allows for sending [msg] and using
+      [state] as the next service state (which in case of [echo] is [tt :
+      unit]). *)
+
+  Goal GenServerNet.echo =
+         {|state_t := unit;
+           init := tt;
+           handle_call from msg st :=
+             reply msg st
+         |}.
+  Proof. reflexivity. Defined.
+
+  (** The more complex service shown below defines [fwd_service], which acts as
+      a proxy by forwarding messages to a [target]. Each message carries a
+      natural number decremented at each forwarding; if [fwd_service] receives
+      0, it instead instantly replies with the number of messages forwarded so
+      far (tracked in the state). The example showcases the auxiliary syntax
+      [let? x := target ! msg' in ]... to perform an RPC call: it sends the
+      query [msg'] to the service [target], awaits a response, and assigns the
+      response payload to the variable [x]. *)
+
+  (** Note that the framework instantiates [Val] with [nat] *)
+  Check valnat : Val = nat.
+
+  Goal GenServerNet.fwd_service = fun (target : string) =>
+      {|state_t := _;
+        init := tt;
+        handle_call (_from : option string) (msg : Val) st :=
+          match valnat_trans msg with
+          | 0 => reply msg st
+          | S msg' =>
+              let? x := target ! msg' in
+              reply x st
+          end
+      |}.
+  Proof. reflexivity. Defined.
+
+
+  (** Initiators are specified by the [InitConf] record with two fields:
+      [target] which names the service to be called; and [msg] for the message
+      to be sent. Networks are assembled by the [gen_net] function based on the
+      provided configuration ([NetConf]) which maps names to initiators and
+      services. Note that initiator names are unrelated to service names, even
+      if they share the same string value: internally, the framework represents
+      them differently and makes it impossible to query an initiator. Because
+      the mapping has to be exhaustive, we use [echo] as a default service and
+      set superfluous initiators to call an unused name. *)
+
+  Print InitConf.
+
+  (** [[
+      Record InitConf : Set := iconf
+      { target : string;
+        msg : Srpc.Locks.Proc.Que.Channel.Val
+      }.
+      ]]
+   *)
+
+  (** Network configuration: *)
+
+  Check gen_net : NetConf -> Net.
+  Print NetConf.
+
+  (** [[
+      Record NetConf :=
+      { services : string -> ServiceConf;
+        inits : string -> InitConf
+      }.
+      ]]
+   *)
+
+  (** All networks generated by [gen_net] contain only SRPC services. *)
+  Check gen_net_SRPC : forall conf n,
+    exists srpc, SrpcDefs.SRPC_serv srpc (NetMod.get n (gen_net conf)).
+
+  (** Moreover, they are [well_formed] *)
   Check gen_well_formed : forall conf, well_formed (gen_net conf).
-  Check gen_KIS : forall conf : NetConf, KIS (gen_instr (gen_net conf)).
-  Check gen_KIC : forall conf : NetConf, KIC (gen_instr (gen_net conf)).
 
-  Check gen_correct : forall conf, detect_correct (gen_net conf) gen_instr.
+  (** We provide an instrumentation [gen_instr] which fulfills our [KIS] and
+  [KIC] invariants. *)
 
-  (** Let's say it again *)
-  Check gen_correct : forall conf,
-      let N0 := gen_net conf in
-      and
-        (forall path' MN1 n,
-            (gen_instr N0 =[ path' ]=> MN1) /\ alarm (MN1 n) = true ->
-            exists DS, In n DS /\ dead_set DS '' MN1
-        )
-        (forall path0' MN1 DS,
-            (gen_instr N0 =[ path0' ]=> MN1) -> dead_set DS '' MN1 ->
-            exists path1' MN2 n,
-              (MN1 =[ path1' ]=> MN2) /\ In n DS /\ alarm (MN2 n) = true
-        ).
-End Correct.
+  Check gen_instr : instr.
+  Check gen_KIS : forall conf, KIS (gen_instr (gen_net conf)).
+  Check gen_KIC : forall conf, KIC (gen_instr (gen_net conf)).
+
+  (** Therefore, networks implemented in this framework can be correctly
+  monitored. *)
+
+  Lemma gen_net_correct : forall conf,
+      CorrectnessCriteria.detect_correct (gen_net conf) gen_instr.
+  Proof. eauto using oopsla_correct, gen_KIS, gen_KIC. Qed.
+
+  (** ** Example network defined in the framework. *)
+  Goal GenServerNet.example_net =
+      gen_net
+        {| services name :=
+            match name with
+            | "C" => fwd_service "B" | "D" => fwd_service "A"
+            | "A" => fwd_service "C" | "B" => fwd_service "D"
+            | _ => GenServerNet.echo
+            end;
+          inits name :=
+            match name with
+            | "iA" => iconf "A" 2 | "iB" => iconf "B" 2
+            | _ => iconf "" 0
+            end
+        |}.
+  Proof. reflexivity. Defined.
+
+  (** It may deadlock! *)
+  Check can_deadlock : exists path N,
+      (example_net =[ path ]=> N) /\ dead_set ["A"; "B"; "C"; "D"]%list N.
+End Framework.
